vyperTestScript.sml
@@ -80,8 +80,26 @@ Definition test_array_assign_ast_def:
     Return (SOME (BinOp (BinOp (Subscript (Name "bar") (Literal (IntL 0))) Add
                                (Subscript (Name "bar") (Literal (IntL 1)))) Add
                         (Literal (IntL 42))))
-
   ]
 End
+
+Theorem evaluate_test_array_assign_body:
+  execute_stmts 10
+    (function_body test_array_assign_ast)
+    initial_function_context = result_ctx
+  ==>
+  result_ctx.raised = SOME (ReturnException (IntV 47))
+Proof
+  rw[function_body_def, test_array_assign_ast_def]
+  \\ simp[execute_stmts_def,
+       initial_function_context_def, new_variable_def,
+       set_variable_def, evaluate_base_target_def, evaluate_target_def,
+       evaluate_exps_def, assign_target_def, add_subscript_def,
+       assign_subscripts_def, extract_elements_def, replace_elements_def,
+       evaluate_cmp_def, evaluate_literal_def, integer_index_def,
+       evaluate_binop_def, push_scope_def, lookup_scopes_def,
+       find_containing_scope_def, pop_scope_def,
+       raise_def, FLOOKUP_UPDATE]
+QED
 
 val () = export_theory();
